GMLInit/Prelude.lean
@@ -1,4 +1,4 @@
-import Std
+import Batteries
 import Extra
 import Logic
 
